lakefile.lean
@@ -20,6 +20,13 @@ require ssreflect from
 lean_lib «LeanMove» where
   -- add any library configuration options here
 
+-- Build target for initial examples
+-- Build with: lake build initial
+lean_lib «initial» where
+  srcDir := "LeanMove/Examples/initial"
+  roots := #[`accepted.borrow_in_loop_fixed_ok, `accepted.deref_borrow_field_ok,
+             `rejected.borrow_in_loop]
+
 -- Build target for expressivity examples
 -- Build with: lake build expressivity
 lean_lib «expressivity» where
@@ -31,3 +38,17 @@ lean_lib «expressivity» where
              `rejected.simple_dangling, `rejected.imm_borrow_after_mut_call_invalid,
              `rejected.imm_borrow_after_mut_fields_invalid,
              `rejected.mutable_borrows_not_unique_calls_invalid]
+
+-- Build all examples
+-- Build with: lake build examples
+lean_lib «examples» where
+  srcDir := "LeanMove/Examples"
+  roots := #[`initial.accepted.borrow_in_loop_fixed_ok, `initial.accepted.deref_borrow_field_ok,
+             `initial.rejected.borrow_in_loop,
+             `expressivity.accepted.alias_write_after_join, `expressivity.accepted.alias_writes,
+             `expressivity.accepted.extension_after_call, `expressivity.accepted.extension_writes_after_join,
+             `expressivity.accepted.imm_borrow_after_mut, `expressivity.accepted.multible_mutable_return_values,
+             `expressivity.accepted.mutable_borrows_are_not_unique, `expressivity.accepted.subtree_writes_release,
+             `expressivity.rejected.simple_dangling, `expressivity.rejected.imm_borrow_after_mut_call_invalid,
+             `expressivity.rejected.imm_borrow_after_mut_fields_invalid,
+             `expressivity.rejected.mutable_borrows_not_unique_calls_invalid]
